\documentclass[11pt]{article}

\usepackage{amsmath} 

\begin{document}
$(x^2+x+1) \times (x-2) = x^3-x^2-x-2$

\newpage

$
\begin{pmatrix} 2\\ 1\\ 0 \end{pmatrix}$ with $\begin{pmatrix} 1\\ x\\ x^2 \end{pmatrix} = x + 2$\\\\

$ \begin{pmatrix} 1\\ 1 \\1 \end{pmatrix}$ with $\begin{pmatrix} 1\\ x\\ x^2 \end{pmatrix} = x^2+x+1$ \hspace{1cm} = $2x^2+2x+4$\\\\

$ \begin{pmatrix} 3\\ 0 \\1 \end{pmatrix}$ with $\begin{pmatrix} 1\\ x\\ x^2 \end{pmatrix} = x^2+1$\

\newpage

\begin{center}
	$3x^2+2x+1$
\end{center}

\newpage

\begin{center}
	\begin{tabular}{l l r}
		$a$ & & $5x^2+15x+10$ \\
		$s$ & $\times$ & $2x^2-4x+2$ \\
		$e$ & $+$ & $-x^2+x-2$  \\ \hline
		$b$ & $=$ & $-10x^2+9x+6$
	\end{tabular}
\end{center}

\end{document}
